State Rewrite laws

src/Refine2.v
@@ -19,22 +19,6 @@ Require Import
   Hask.Control.Monad
   RWS.
 
-
-Program Definition denotes_state {effs v}: Eff (State state :: effs) v -> Eff effs v -> Prop :=
-    handleRelayP
-      (fun x e => match e with
-               | Pure x' =>  x = x'
-               | Impure u k => False
-               end)
-      (fun V (st: State state V) a =>
-         match st in State _ a' return V = a' -> _ with
-         | Get => fun _ => True
-         | Put x => _
-         end eq_refl).
-Next Obligation.
-refine (forall y, x y = 2).
-Defined.
-
 Fixpoint denote_aexp `{Member (State state) effs}
          (a:aexp): Eff effs nat :=
   match a with
@@ -109,36 +93,19 @@ Eval cbn in swap_spec1.
  2) put s' >>= put s =~= put s
  3) put s >>= get =~= s
 *)
-Definition state_default: forall eff r, FindElem eff [State state] -> eff r -> r.
-  intros.
-  inversion X; subst.
-  inversion X0; subst.
-  refine (t_empty 0).
-  refine tt.
-  inversion X1.
-Defined.
-
-Definition state_size {v} (e: Eff [State state] v): nat := Eff_size e state_default.
-
-Eval compute in (state_size swap_spec1).
-Eval compute in (state_size swap_spec2).
-Eval compute in (state_size (denote_imp swap_impl)).
-
-Open Scope bool_scope.
 
 Fixpoint opt_getget' (b: bool) (s: state) `(e: Eff [State state] v): Eff [State state]  v :=
   match e with
    | Pure x => pure x
    | Impure u k =>
-     let default := fun b' s' x => opt_getget' b' s' (k x) in
      match extract u in State _ s return s = _ -> _ with
-     | Get => fun Heq => if b then default true s (rew [id] Heq in s)
-             else Impure u (fun x => default true s x)
-     | Put x => fun _ => Impure u (default false s)
+     | Get => fun Heq => if b
+                     then opt_getget' true s (k (rew [id] Heq in s))
+                     else Impure u (fun x => opt_getget' true (rew <- [id] Heq in x) (k x))
+     | Put x => fun _ => Impure u (fun x => opt_getget' false s (k x))
      end eq_refl
   end.
 Definition opt_getget {v} := @opt_getget' false (t_empty 0) v.
-
 
 Fixpoint opt_putput `(e: Eff [State state] v): Eff [State state] v :=
    match e with
@@ -170,15 +137,32 @@ Fixpoint opt_putget `(e: Eff [State state] v): Eff [State state] v :=
                                | Pure x' => Pure x'
                                | @Impure _ _ T' u' k' =>
                                  match extract u' in State _ s return s = T' -> _ with
-                                 | Put st' => fun _ => opt_putget (k x)
+                                 | Put st' => fun _ => Impure u' (fun x' => opt_putget (k' x'))
                                  | Get => fun Heq' => opt_putget (k' (rew [id] Heq' in st))
                                  end eq_refl
                                end)
-                            
      end eq_refl
    end.
 
 Definition step_opt {v} := @opt_putget v \o @opt_getget v \o @opt_putput v.
+
+(* Now to run these laws until we hit a normal formal we need will need the notion
+ * of sizes of our terms.
+ *)
+Definition state_default: forall eff r, FindElem eff [State state] -> eff r -> r.
+  intros.
+  inversion X; subst.
+  inversion X0; subst.
+  refine (t_empty 0).
+  refine tt.
+  inversion X1.
+Defined.
+
+Definition state_size {v} (e: Eff [State state] v): nat := Eff_size e state_default.
+
+Eval compute in (state_size swap_spec1).
+Eval compute in (state_size swap_spec2).
+Eval compute in (state_size (denote_imp swap_impl)).
 
 Program Fixpoint opt `(e: Eff [State state] v) {measure (state_size e)} :=
   let step := step_opt e in
@@ -187,40 +171,23 @@ Program Fixpoint opt `(e: Eff [State state] v) {measure (state_size e)} :=
   | _ => step
   end.
 
-Definition swap_spec1_opt: Eff [State state] unit :=
-  (opt swap_spec1).
-
-Definition swap_spec2_opt: Eff [State state] unit :=
-  (opt swap_spec2).
-
-Definition swap_impl_opt: Eff [State state] unit :=
-  (opt (denote_imp swap_impl)).
-
-Eval cbn in ((denote_imp swap_impl)).
-(* There is a bug on put put *)
-Eval cbn in (swap_spec1_opt).
-Eval cbn in (swap_impl_opt).
-Eval cbn in (swap_spec2_opt).
-(* I need to apply this function multiple times now, until the term normalizes.
-What can I do? *)
-Eval cbn in (opt swap_spec2_opt).
-Eval cbn in (opt swap_impl_opt).
-
-Definition refines {a effs} (e1 e2: Eff effs a) := 
-  forall t, e2 = t -> e1 = t.
+Definition refines {a} (e1 e2: Eff [State state] a) := 
+  opt e1 = opt e2.
 
 Lemma swap_impl_respects_spec2:
-  opt swap_impl_opt = opt swap_spec2_opt.
+  refines (denote_imp swap_impl) swap_spec2.
 Proof.
   reflexivity.
 Qed.
 
 Lemma swap_impl_respects_spec1:
-  swap_impl_opt = swap_spec1_opt.
+  refines (denote_imp swap_impl) swap_spec1.
 Proof.
   reflexivity.
 Qed.
 
-
-
-
+Lemma swap_spec1_respects_spec2:
+  refines swap_spec1 swap_spec2.
+Proof.
+  reflexivity.
+Qed.
